examples/dynamic_isolation/Proof.v
@@ -1,0 +1,194 @@
+Require Import Koika.Frontend.
+Require Import Coq.Lists.List.
+
+Require Import Koika.Std.
+
+Require Import DynamicIsolation.Interfaces.
+Require Import DynamicIsolation.External.
+Require Import DynamicIsolation.Multicore.
+
+Module Pf (External: External_sig) (EnclaveParams: EnclaveParameters)
+          (Params0: CoreParameters) (Params1: CoreParameters)
+          (Core0: Core_sig External EnclaveParams Params0)
+          (Core1: Core_sig External EnclaveParams Params1)
+          (Memory: Memory_sig External).
+  Module Impl:= MachineSemantics External EnclaveParams Params0 Params1 Core0 Core1 Memory.
+  Import Common.
+  Import Interfaces.Common.
+
+  Record enclave_metadata :=
+    { meta_eid : enclave_id;
+      shared_page : bool
+    }.
+
+  Record enclave_params :=
+    { metadata : enclave_metadata;
+      param_dram: initial_dram_t
+    }.
+
+  Record core_config : Type :=
+    { enclave_data : enclave_metadata;
+      in_limbo: bool;
+      requested_enclave: option enclave_metadata;
+      state_fn : nat -> observations_t
+    }.
+
+  Definition rf_t : Type := env_t ContextEnv Rf.R.
+
+  Definition isolated_function_t : Type := ind_core_id -> enclave_params -> rf_t -> nat -> observations_t.
+
+  Record partitioned_memory :=
+    { pm_enclave_mem : enclave_id -> option initial_dram_t;
+      pm_shared_page : option initial_dram_t;
+    }.
+
+  Record ghost_state :=
+    { core0_config : core_config;
+      core1_config : core_config;
+      mem_partitions : partitioned_memory;
+      num_cycles : nat
+    }.
+
+
+  (* TODO: This should be derived from Interfaces *)
+  Definition initial_rf : rf_t := ContextEnv.(create) Rf.r.
+
+  Definition mk_initial_config (fn: isolated_function_t) (core_id: ind_core_id)
+                               (params: enclave_params) (rf: rf_t) : core_config :=
+    {| enclave_data := params.(metadata);
+       in_limbo := false;
+       requested_enclave := None;
+       state_fn := fn core_id params rf
+    |}.
+
+  Definition enclave_base enc_id := Bits.to_nat (EnclaveParams.enclave_base enc_id).
+  Definition enclave_max enc_id := Bits.to_nat (Bits.plus (EnclaveParams.enclave_base enc_id)
+                                                          (EnclaveParams.enclave_size enc_id)).
+
+  Definition initial_enclave_dram initial_dram enc_id : initial_dram_t :=
+    fun addr => if ((enclave_base enc_id) <=? addr) && (addr <? (enclave_max enc_id))
+             then initial_dram addr
+             else None.
+
+  Definition initial_shared_mem initial_dram : initial_dram_t :=
+    fun addr => if ((Bits.to_nat (EnclaveParams.shared_mem_base) <=? addr) &&
+                 (addr <? Bits.to_nat (Bits.plus EnclaveParams.shared_mem_base EnclaveParams.shared_mem_size)))
+             then initial_dram addr
+             else None.
+
+  Definition mk_initial_pm (initial_dram: initial_dram_t) : partitioned_memory :=
+    {| pm_enclave_mem := fun eid => Some (initial_enclave_dram initial_dram eid);
+       pm_shared_page := Some (initial_shared_mem initial_dram)
+    |}.
+
+  Definition initial_ghost_state (fn: isolated_function_t) (initial_dram: initial_dram_t) : ghost_state :=
+    let enclave0_param :=
+        {| metadata := {| meta_eid := Enclave0;
+                          shared_page := false
+                       |};
+           param_dram := initial_enclave_dram initial_dram Enclave0
+        |} in
+    let enclave1_param :=
+        {| metadata := {| meta_eid := Enclave1;
+                          shared_page := false
+                       |};
+           param_dram := initial_enclave_dram initial_dram Enclave1
+        |} in
+    {| core0_config := mk_initial_config fn CoreId0 enclave0_param initial_rf;
+       core1_config := mk_initial_config fn CoreId1 enclave1_param initial_rf;
+       mem_partitions := {| pm_enclave_mem := fun eid => match eid with
+                                                      | (Enclave0 | Enclave1) => None
+                                                      | _ => Some (initial_enclave_dram initial_dram eid)
+                                                      end;
+                            pm_shared_page := Some (initial_shared_mem initial_dram)
+                         |};
+       num_cycles := 0
+    |}.
+
+  (* TODO: Do we care about cycle-accurate purge? *)
+  Inductive function_generates_trace_helper
+            (fn: isolated_function_t) (initial_dram: initial_dram_t)
+            (ghost: ghost_state) (tr: trace) : Prop :=
+  | EmptyTrace :
+      forall (initial_ghost : ghost = initial_ghost_state fn initial_dram)
+        (empty_trace: tr = []),
+      function_generates_trace_helper fn initial_dram ghost tr
+  | IndTrace_BothRunning :
+      forall (prev_tr: trace) (obs: ind_core_id -> observations_t)
+        (prev_ghost: ghost_state) (ghost0 ghost1: ghost_state)
+
+        (* Induction hypothesis *)
+        (ind_hyp: function_generates_trace_helper fn initial_dram prev_ghost prev_tr)
+        (* If Core0 is running an enclave,
+         * fn must generate the relevant observation
+         *)
+        (pf_case_core0_running : prev_ghost.(core0_config).(in_limbo) = false ->
+                                 obs CoreId0 = prev_ghost.(core0_config).(state_fn) (S prev_ghost.(num_cycles))
+        )
+        (* If Core0 is not running an enclave *)
+        (pf_case_core0_limbo : prev_ghost.(core0_config).(in_limbo) = true ->
+                               obs CoreId0 = prev_ghost.(core0_config).(state_fn) (S prev_ghost.(num_cycles))
+        )
+
+
+        (* If Core1 is running an enclave *)
+        (* If Core1 is not running an enclave *)
+
+
+        (core0_running : prev_ghost.(core0_config).(in_limbo) = false)
+        (core1_running : prev_ghost.(core1_config).(in_limbo) = false)
+        (trace_eq: tr = prev_tr ++ [obs]),
+        (*
+        (ghost0_eq: ghost0 =
+        (ghost1_eq: ghost1 =
+
+        (cur_obs.obs_enclave_req
+        *)
+        (* TODO *)
+      function_generates_trace_helper fn initial_dram ghost tr.
+
+
+
+  Definition function_generates_trace (fn: isolated_function_t) (initial_dram: initial_dram_t) (tr: trace) : Prop :=
+    exists ghost_state, function_generates_trace_helper fn initial_dram ghost_state tr.
+
+
+  Section Initialised.
+    Variable initial_dram: initial_dram_t.
+
+    Theorem simulation: exists (iso_fn : isolated_function_t),
+      forall (n: nat) (impl_st: Impl.state) (impl_tr: trace),
+        Impl.step_n initial_dram n = (impl_st, impl_tr) ->
+        function_generates_trace iso_fn initial_dram impl_tr.
+    Admitted.
+
+  End Initialised.
+
+End Pf.
+
+
+
+Module OldPf (External: External_sig) (EnclaveParams: EnclaveParameters)
+          (Params0: CoreParameters) (Params1: CoreParameters)
+          (Core0: Core_sig External EnclaveParams Params0)
+          (Core1: Core_sig External EnclaveParams Params1)
+          (Memory: Memory_sig External).
+  Module Impl:= MachineSemantics External EnclaveParams Params0 Params1 Core0 Core1 Memory.
+  Module Spec:= IsolationSemantics External EnclaveParams Params0 Params1 Core0 Core1 Memory.
+
+  Import Common.
+
+  Section Initialised.
+    Variable initial_dram: initial_dram_t.
+
+    Theorem simulation: forall (n: nat)
+                          (impl_st: Impl.state) (impl_tr: trace)
+                          (spec_st: Spec.state) (spec_tr: trace),
+        Impl.step_n initial_dram n = (impl_st, impl_tr) ->
+        Spec.step_n  initial_dram n = (spec_st, spec_tr) ->
+        impl_tr = spec_tr.
+     Admitted.
+
+  End Initialised.
+
+End OldPf.
